New method : terms are functions

Notations.v
@@ -9,167 +9,229 @@ Declare Custom Entry expr.
 Declare Custom Entry type.
 
 (* Entry point *)
-Notation "[| x |]" := x (x custom expr at level 2).
-Notation "( x )" := x (in custom expr, x custom expr).
-Notation "|[ x ]|" := x (in custom expr, x constr).
-Notation "x" := x (in custom expr at level 0, x ident).
+
+Notation "'|' t" := (fun (fv_id:nat) => t) (at level 200).
+Notation "[| x |]" := (x 0) (x custom expr at level 2).
+Notation "( x )" := (fun (fv_id:nat) => (x fv_id)) (in custom expr, x custom expr).
+Notation "x" := (fun fv_id => x) (in custom expr at level 0, x ident). 
 
 (* Variables (nameless) *)
-Notation "'ft{' v '}'" := (fvar v term_var) (in custom expr,
+Notation "'ft{' v '}'" := (| (fvar v term_var)) (in custom expr,
                                                 v constr).
-Notation "'fT{' t '}'" := (fvar t type_var) (in custom type,
-                                                t constr).
-Notation "'lt{' v '}'" := (lvar v term_var) (in custom expr,
+Notation "'lt{' v '}'" := (| (lvar v term_var)) (in custom expr,
                                                 v constr).
-Notation "'lT{' t '}'" := (lvar t type_var) (in custom type at level 4,
-                                                t constr at level 4).
+
+
+Notation "( t1 , t2 )" :=
+  (fun fv_id => (pp (t1 fv_id) (t2 fv_id)))
+  (in custom expr, t1 custom expr, t2 custom expr).
+
+Notation "'0'" := (| zero) (in custom expr).
+
+Notation "'fun' => t" :=
+     (fun fv_id => (
+          (notype_lambda (t fv_id))))
+     (in custom expr at level 100, t custom expr).
+Notation "'fun' ( x ) => t" :=
+     (fun fv_id => (
+          let x := (fvar fv_id term_var) in
+          (notype_lambda (close 0 (t (S fv_id)) fv_id))))
+     (in custom expr at level 100, x ident, t custom expr).
+
+Notation "'fun' f ( x ) => t" :=
+     (fun fv_id => (
+          let x := (fvar fv_id term_var) in
+          (notype_lambda (close 0 (t (S fv_id)) fv_id))))
+     (in custom expr at level 100, f ident, x ident, t custom expr).
+
+Notation "'def_rec' f x => t":=
+     (fun fv_id => (
+        let f := (fvar fv_id term_var) in
+        let x := (fvar (S fv_id) term_var) in
+        (notype_tfix (close 0 (notype_lambda (close 0 (t (S (S fv_id))) (S fv_id))) fv_id) )))
+     (in custom expr at level 100, f ident, x ident, t custom expr).
+
+Notation "'def_rec' f x y => t":=
+     (fun fv_id => (
+          let f := (fvar fv_id term_var) in
+          let x := (fvar (S fv_id) term_var) in
+          let y := (fvar (S (S fv_id)) term_var) in
+          (notype_tfix (
+             close 0 (
+               notype_lambda (
+                 close 0 (
+                    notype_lambda (
+                        close 0 (
+                          t (S(S(S fv_id))))
+                        (S (S fv_id))))
+                 (S fv_id)))
+             fv_id))))
+     (in custom expr at level 100, f ident, x ident, y ident, t custom expr).
+
+Notation " t1 t2 " :=
+  (fun fv_id => (app (t1 fv_id) (t2 fv_id)))
+    (in custom expr at level 200, right associativity,
+        t1 custom expr,
+        t2 custom expr).
+
+Eval compute in [| fun f (x) => (fun g (y) => (x,y)) |].
+
+Eval compute in [| def_rec plus x y => ((plus, x), y) |].
+Eval compute in [| fun set_left (x) => (x, 0) |].
+Eval compute in [| fun truc(x) => (fun truc2(y) => (fun truc3(z) => ((x,y),z))) |].
+
+Eval compute in [| ((ft{0}, 0), 0) |].
+
 (* Untyped language *)
 (* --------------------------------------------------------------------- *)
 
-Notation "'()'" := (uu) (in custom expr).
+Notation "'()'" := (|uu) (in custom expr).
 
-Notation "'size' ( t )" := (tsize t) (in custom expr at level 1,
-                                         t custom expr at level 4).
+Eval compute in [| () |].
 
+Notation "'size' ( t )" := (fun fv_id => (tsize (t fv_id))) (in custom expr,
+                                         t custom expr).
 
-Notation "'fun' => y" := (notype_lambda y) (in custom expr at level 4,
-                                              y custom expr at level 4).
-Notation "'def' f : y" := (notype_lambda y) (in custom expr at level 100,
-                                                f ident,
-                                                y custom expr at level 4).
-Notation " t1 t2 " := (app t1 t2) (in custom expr at level 2,
-                                      t1 custom expr,
-                                      t2 custom expr at level 4).
 (* Pairs *)
 
-Notation "( t1 , t2 , .. , tn )" := (pp .. (pp t1 t2) .. tn) (in custom expr,
-                                           t1 custom expr,
-                                           t2 custom expr,
-                                           tn custom expr).
-Notation "t '._1'" := (pi1 t) (in custom expr at level 2,
+Notation "t '._1'" := (fun fv_id => (pi1 (t fv_id))) (in custom expr at level 200,
                                   t custom expr).
-Notation "t '._2'" := (pi2 t) (in custom expr at level 2,
+Notation "t '._2'" := (fun fv_id => (pi2 (t fv_id))) (in custom expr at level 200,
                                   t custom expr).
 
 (* Booleans *)
-Notation "'true'" := (ttrue) (in custom expr).
-Notation "'false'" := (tfalse) (in custom expr).
-Notation "'if' c 'then' t 'else' f" := (ite c t f) (in custom expr at level 1,
-                                                       c custom expr at level 2,
-                                                       t custom expr at level 4,
-                                                       f custom expr at level 4).
+Notation "'true'" := (|ttrue) (in custom expr).
+Notation "'false'" := (|tfalse) (in custom expr).
+Notation "'if' c 'then' t 'else' f" := (fun fv_id => (ite (c fv_id) (t fv_id) (f fv_id))) (in custom expr at level 1,
+                                                       c custom expr,
+                                                       t custom expr,
+                                                       f custom expr).
 
 (* Naturals *)
-Notation "'0'" := zero (in custom expr).
-Notation "'1'" := (succ zero) (in custom expr).
-Notation "'s' t" := (succ t) (in custom expr at level 2,
+Notation "'1'" := (| (succ zero)) (in custom expr).
+Notation "'s' t" := (fun fv_id => (succ (t fv_id))) (in custom expr at level 2,
                                  t custom expr).
-Notation " t 'match'  '|' t1 '|' t2 'end'" := (tmatch t t1 t2) (in custom expr at level 2,
-                                                              t1 custom expr at level 4,
-                                                              t2 custom expr).
 
-(* Fix points *)
-(* Notation "'fix' t" := (notype_tfix t) (in custom expr at level 2,
-                                          t custom expr).
-*)
+Notation "'match' t 'with' '|' '0' => t1 '|' 's' x => t2 'end'" :=
+  (fun (fv_id:nat) => (
+       tmatch (t fv_id)
+              (t1 fv_id)
+              (let x := (fvar fv_id term_var) in (close 0 (t2 (S fv_id)) fv_id))))
+  (in custom expr at level 190,
+      t custom expr,
+      t1 custom expr,
+      t2 custom expr,
+      x ident).
+
+Eval compute in
+    [| match 0 with
+         |0 => 1
+         |s n => (
+            match n with
+            | 0 => 0
+            | s n' => n' end) end |].
+
+Definition sfr_plus := [|
+ def_rec plus x y =>
+ (match x with
+     | 0 => y
+     | s x' => (plus x' y) end)
+|].
+
+Example ex1 : wf sfr_plus 0.
+Proof.
+  repeat step.
+Qed.
+
 (* Let expression *)
-Notation "'let' := t1 'in' t2" := (notype_tlet t1 t2) (in custom expr at level 1,
-                                                       t1 custom expr at level 4,
-                                                       t2 custom expr at level 4).
+Notation "'let' x := t1 'in' t2" :=
+  (fun (fv_id : nat) => (
+       notype_tlet (t1 fv_id)
+                   (let x := (fvar fv_id term_var) in (close 0 (t2 (S fv_id)) fv_id) )))
+    (in custom expr at level 190,
+        t1 custom expr,
+        t2 custom expr,
+        x ident).
+
+Check
+    [| let n := 1 in (match n with
+                                 | 0 => 1
+                                 | s n' => (match n' with
+                                             | 0 => 1
+                                             | s n'' => ((n, n'),n'') end) end) |].
+
+Eval compute in
+[|
+ let plus := (def_rec f x y => (match x with
+                                    | 0 => y
+                                    | s x' => (f x' y) end)) in (
+ let fibo := (def_rec f n => (match n with
+                                 | 0 => 1
+                                 | s n' => (match n' with
+                                             | 0 => 1
+                                             | s n'' => plus (f n') (f n'') end) end))
+                 in fibo (s (s (s (s (s 0))))))
+|].
+
+
 (* Sum *)
-Notation "'right' ( t )" := (tright t) (in custom expr at level 2,
-                                         t custom expr at level 4).
-Notation "'left' ( t )" := (tleft t) (in custom expr at level 2,
-                                         t custom expr at level 4).
-Notation "t 'match' '|' 'left' => t1 '|' 'right' => t2 'end'" := (sum_match t t1 t2) (in custom expr at level 2,
-                                                                                       t custom expr,
-                                                                                       t1 custom expr,
-                                                                                       t2 custom expr).
+Notation "'right' t " :=
+  (fun fv_id => tright (t fv_id))
+  (in custom expr at level 180, right associativity, t custom expr).
+Notation "'left' t " := 
+  (fun fv_id => tleft (t fv_id))
+  (in custom expr at level 180, right associativity, t custom expr).
 
-Notation "'fun' [ T ] => y" := (lambda T y) (in custom expr at level 4,
-                                               T custom type at level 4,
-                                               y custom expr at level 4).
 
-Definition fresh_id (t: tree) := makeFresh (fv t :: nil).
-
-Notation "'fun' ( x ) => t" :=
-   (let fresh := (S (let x := (fvar 0 term_var) in (max (fv t)))) in 
-    let x     := (fvar fresh term_var) in
-    notype_lambda (close 0 t fresh))
-     (in custom expr at level 100, x ident, t custom expr).
+Notation "'match' t 'with' '|' 'left' l => t1 '|' 'right' r => t2 'end'" :=
+  (fun (fv_id:nat) => (
+       tmatch (t fv_id)
+              (let l  := (fvar fv_id term_var) in (close 0 (t1 (S fv_id)) fv_id))
+              (let r := (fvar fv_id term_var) in (close 0 (t2 (S fv_id)) fv_id))))
+  (in custom expr at level 190,
+      t custom expr,
+      t1 custom expr,
+      t2 custom expr,
+      l ident,
+      r ident).
 
 Eval compute in [| fun ( x ) => x |].
 
-  (*
-Notation "'fun' ( x ) => t" :=
-   (let fresh := fresh_id (let x := (fvar 0 term_var) in t) in
-   ((fun x => (fvar fresh term_var))
-   (notype_lambda (close 0 t fresh)))) (in custom expr at level 100, x ident, t custom expr). *)
-
 Eval compute in [| fun ( x ) => (fun (y) => x) |].
-Example test1 : [| fun ( x ) => (x, (fun (y) => (x, y)), x) |] = [| fun => ((lt{0}, (fun => (lt{1}, lt{0}))), lt{0}) |].
+Example test1 : [| fun ( x ) => ((x, fun (y) => (x, y)), x) |] = [| fun => ((lt{0}, (fun => (lt{1}, lt{0}))), lt{0}) |].
 Proof.
-  unfold fv, pfv, max.
-  simpl.
-  assert (forall t:nat, (if tag_eq_dec term_var term_var then singleton t else nil) = (singleton t)) as H. {
-    destruct (tag_eq_dec term_var term_var) eqn:E.
-    reflexivity.
-    congruence. }
-  rewrite ?H.
-  simpl.
-  reflexivity.
-Qed.
+  repeat step.
+  Qed.
 
 Eval compute in [| fun ( x ) => (fun (y) => x)|].
-
-Notation "'def_rec' f '(' x ')' := t" :=
-  (let f := (fvar 1000 term_var) in
-   let x := (fvar 999 term_var) in
-   (notype_tfix (close 0 (close 1 t 999) 1000)))
-  (in custom expr at level 100, f ident, x ident, t custom expr, right associativity).
-
 
 
 Eval compute in [|
      fun (x) => (fun (y) => ((x,y), fun(z) => (x, y))) |].
 
-Eval compute in [|
-(
-def_rec plus(pair) :=
-  pair._1 match
-    | pair._2
-    | fun(x) => s (plus (x, pair._2))
-  end
-) (0, 0)
-|].
-
-Notation "'λ' f" := (notype_lambda (close 0 (f (fvar 1000 term_var)) 1000))
-  (at level 300, right associativity).
-
-Eval compute in (λ (fun x => (pp x (notype_lambda x)))).
 (* Examples *)
 (* --------------------------------------------------------------------- *)
 
 (* Unset Printing Notations. *)
 
-Example ex1: wf [| if true then 0 else 1 |] 0.
+Example ex11: wf [| if true then 0 else 1 |] 0.
 Proof. repeat step. Qed.
 
 Example ex2: wf [|
-                 fun => lt{0} match
-                       | left => 0
-                       | right => 1 end
+                 fun => match lt{0} with
+                       | left x => 0
+                       | right x => 1 end
                 |] 0.
 Proof. repeat step. Qed.
 
 Example ex3: wf [|
-                 fun => let := (s 1) in
-                     if lt{0} then (
-                         lt{1} match
-                           | 1
-                           | (fun => (s lt{2})) end)
+                 fun => let x := (s 1) in
+                     if x then (
+                         match 0 with
+                           | 0 => 1
+                           | s _ => x  end)
                      else (
-                         let := 0 in ()
+                         let y := 0 in ()
                        )
                  |] 0.
 Proof. repeat step. Qed.
@@ -177,14 +239,6 @@ Proof. repeat step. Qed.
 (* close free variable -> local variable *)
 
 
-Compute tree_size [|
-         let zero := s 0 in lt{0} match
-         | s 0
-             | s (s 0) end
-|].
-
-
-Compute close 0 (notype_lambda ((fvar 5 term_var))) 5.
 
 
 
